Complete the first version of map decide; next is existentials

Lib/MapDecide.v
@@ -7,321 +7,30 @@ Require Import Category.Lib.Nomega.
 Require Import Category.Lib.FMapExt.
 
 Generalizable All Variables.
+Set Transparent Obligations.
+
+(* For the time being, this module is fixed to maps from [N * N -> N]. *)
 
 Module PO := PairOrderedType N_as_OT N_as_OT.
 Module M  := FMapList.Make(PO).
 Module Import FMapExt := FMapExt PO M.
 
-Notation "[map ]" := (M.empty _) (at level 9, only parsing).
-Notation "x +=> y" := (M.add x y) (at level 9, y at level 100, only parsing).
-Notation "[map  a ; .. ; b ]" := (a .. (b [map]) ..) (only parsing).
+(**************************************************************************
+ * Data type for representing partial results, taken from Chlipala's CPDT
+ *)
 
-Lemma mapsto_inv : ∀ elt f g (fg : elt) x y z m,
-  M.MapsTo (f, g) fg (M.add (x, y) z m) ->
-    (x = f ∧ y = g ∧ z = fg) ∨ M.MapsTo (f, g) fg m.
-Proof.
-  intros.
-  apply add_mapsto_iffT in H.
-  destruct H; simpl in *; intuition.
-Defined.
+Inductive partial (P : Prop) : Set :=
+| Proved : P -> partial P
+| Uncertain : partial P.
 
-Lemma find_inv : ∀ f g (fg : N) x y z m,
-  M.find (f, g) (M.add (x, y) z m) = Some fg ->
-    (x = f ∧ y = g ∧ z = fg) ∨ M.find (f, g) m = Some fg.
-Proof.
-  intros.
-  destruct (N.eq_dec x f).
-    destruct (N.eq_dec y g).
-      destruct (N.eq_dec z fg).
-        subst; left; intuition.
-      contradiction n.
-      rewrite F.add_eq_o in H.
-        inversion_clear H.
-        reflexivity.
-      simpl; intuition.
-    rewrite F.add_neq_o in H; intuition.
-  rewrite F.add_neq_o in H; intuition.
-Defined.
-
-Global Program Instance sigT_proper {A : Type} :
-  Proper (pointwise_relation A Basics.arrow ==> Basics.arrow) (@sigT A).
-Next Obligation.
-  proper.
-  destruct X0.
-  apply X in x1.
-  exists x0.
-  assumption.
-Defined.
-
-Lemma find_mapsto_iff_ex {elt k m} :
-  (∃ v : elt, M.MapsTo (elt:=elt) k v m) ->
-  (∃ v : elt, M.find (elt:=elt) k m = Some v).
-Proof.
-  apply sigT_proper.
-  intros ??.
-  apply F.find_mapsto_iff.
-  assumption.
-Defined.
-
-Ltac destruct_maps :=
-  repeat match goal with
-  | [ H : M.find (?X, ?Y) (M.empty _) = Some ?F |- _ ] =>
-    inversion H
-  | [ H : M.find (?X, ?Y) (M.add _ _ _) = Some ?F |- _ ] =>
-    apply find_inv in H;
-    (destruct H as [[? [? ?]]|]; [subst; try nomega|])
-  | [ |- ∃ v, M.find _ _ = Some v ] =>
-    vm_compute; eexists; reflexivity
-
-  | [ H : M.find _ _ = Some _ |- _ ] =>
-    apply F.find_mapsto_iff in H
-  | [ |- M.find _ _ = Some _ ] =>
-    apply F.find_mapsto_iff
-  | [ |- ∃ v, M.find _ _ = Some v ] =>
-    apply find_mapsto_iff_ex
-
-  | [ H : M.MapsTo _ _ (M.empty _) |- _ ] =>
-    contradiction (proj1 (F.empty_mapsto_iff _ _) H)
-
-  | [ H : M.MapsTo (?X, ?Y) ?F (M.add _ _ _) |- _ ] =>
-    apply mapsto_inv in H; destruct H as [[? [? ?]]|]
-
-  | [ H : ?X = ?Y |- context[M.MapsTo (?Y, _)] ] =>
-    rewrite <- H; cbn
-  | [ H : ?X = ?Y |- context[M.MapsTo (_, ?Y)] ] =>
-    rewrite <- H; cbn
-  | [ H : ?X = ?Y |- context[M.MapsTo _ ?Y] ] =>
-    rewrite <- H; cbn
-
-  | [ |- ∃ _, M.MapsTo (?X, ?Y) _ _ ] =>
-    match goal with
-      [ |- context[M.add (X, Y) ?F _ ] ] =>
-      exists F
-    end
-  | [ |- M.MapsTo (?X, ?Y) ?F (M.add (?X, ?Y) ?F _) ] =>
-    simplify_maps
-  | [ |- M.MapsTo _ _ (M.add _ _ _) ] =>
-    simplify_maps; right; split; [idtac|]
-  end;
-  try congruence.
-
-Local Obligation Tactic := simpl; intros.
-
-Lemma peano_rect' : ∀ P : N → Type, P 0%N → (∀ n : N, P (N.succ n)) → ∀ n : N, P n.
-Proof.
-  intros.
-  induction n using N.peano_rect.
-    apply X.
-  apply X0.
-Defined.
-
-Inductive term :=
-  | Var : positive -> term
-  | Value : N -> term.
-
-Definition term_beq (x y : term) : bool :=
-  match x, y with
-  | Var x, Var y => (x =? y)%positive
-  | Value x, Value y => (x =? y)%N
-  | _, _ => false
-  end.
-
-Lemma term_beq_sound x y : term_beq x y = true -> x = y.
-Proof.
-  induction x, y; simpl; intros; intuition.
-  - apply Pos.eqb_eq in H; subst; reflexivity.
-  - apply N.eqb_eq in H; subst; reflexivity.
-Defined.
-
-Program Definition term_eq_dec (x y : term) : {x = y} + {x ≠ y} :=
-  match x, y with
-  | Var x,   Var y   => if Pos.eq_dec x y then left _ else right _
-  | Value x, Value y => if N.eq_dec   x y then left _ else right _
-  | _, _ => right _
-  end.
-Next Obligation. congruence. Defined.
-Next Obligation. congruence. Defined.
-Next Obligation. congruence. Defined.
-Next Obligation. congruence. Defined.
-Next Obligation.
-  destruct H.
-  destruct x, y, wildcard', wildcard'0; try discriminate.
-    specialize (H0 p1 p2).
-    intuition.
-  specialize (H n1 n2).
-  intuition.
-Defined.
-Next Obligation.
-  split; intros;
-  unfold not; intros;
-  destruct H1;
-  discriminate.
-Defined.
-Next Obligation.
-  split; intros;
-  unfold not; intros;
-  destruct H1;
-  discriminate.
-Defined.
-
-Lemma K_dec_on_type A (x : A) (eq_dec : ∀ y : A, x = y \/ x ≠ y)
-      (P : x = x -> Type) :
-  P (eq_refl x) -> forall p:x = x, P p.
-Proof.
-  intros.
-  elim (@Eqdep_dec.eq_proofs_unicity_on A _) with x (eq_refl x) p.
-    trivial.
-  exact eq_dec.
-Qed.
-
-Lemma Pos_eq_dec' : ∀ x y : positive, x = y \/ x ≠ y.
-Proof.
-  intros.
-  destruct (Pos.eq_dec x y); auto.
-Qed.
-
-Lemma Pos_eq_dec_refl n : Pos.eq_dec n n = left (@eq_refl positive n).
-Proof.
-  destruct (Pos.eq_dec n n).
-    refine (K_dec_on_type positive n (Pos_eq_dec' n)
-              (fun x => @left _ _ x = @left _ _ (@eq_refl positive n)) _ _).
-    reflexivity.
-  contradiction.
-Qed.
-
-Lemma N_eq_dec' : ∀ x y : N, x = y \/ x ≠ y.
-Proof.
-  intros.
-  destruct (N.eq_dec x y); auto.
-Qed.
-
-Lemma N_eq_dec_refl n : N.eq_dec n n = left (@eq_refl N n).
-Proof.
-  destruct (N.eq_dec n n).
-    refine (K_dec_on_type N n (N_eq_dec' n)
-              (fun x => @left _ _ x = @left _ _ (@eq_refl N n)) _ _).
-    reflexivity.
-  contradiction.
-Qed.
-
-Lemma prod_eq_dec' :
-  ∀ (A B : Type) (A_eq_dec : ∀ x y : A, x = y ∨ x ≠ y)
-    (B_eq_dec : ∀ x y : B, x = y ∨ x ≠ y)
-    (x y : A ∧ B), x = y \/ x ≠ y.
-Proof.
-  intros.
-  destruct x, y; simpl.
-  destruct (A_eq_dec a a0); subst.
-    destruct (B_eq_dec b b0); subst.
-      left; reflexivity.
-    right; congruence.
-  right; congruence.
-Qed.
-
-Lemma prod_eq_dec_refl (A B : Type) n
-      (A_eq_dec : ∀ x y : A, x = y ∨ x ≠ y)
-      (B_eq_dec : ∀ x y : B, x = y ∨ x ≠ y) :
-  prod_eq_dec A_eq_dec B_eq_dec n n = left (@eq_refl (A ∧ B) n).
-Proof.
-  destruct (prod_eq_dec _ _ n n).
-    refine (K_dec_on_type (A ∧ B) n (prod_eq_dec' _ _ A_eq_dec B_eq_dec n)
-              (fun x => @left _ _ x = @left _ _ (@eq_refl (A ∧ B) n)) _ _).
-    reflexivity.
-  contradiction.
-Qed.
-
-Lemma length_remove A (A_eq_dec : ∀ x y : A, x = y ∨ x ≠ y) x xs :
-  (length (remove A_eq_dec x xs) <= length xs)%nat.
-Proof.
-  induction xs; auto.
-  simpl.
-  destruct (A_eq_dec x a); subst.
-    apply Nat.le_le_succ_r, IHxs.
-  simpl.
-  apply le_n_S, IHxs.
-Qed.
-
-Definition lookup_definition (defs : list (positive * N))
-           (x : positive) : option N :=
-  match find (fun p => fst p =? x)%positive defs with
-  | Some v => Some (snd v)
-  | None => None
-  end.
-
-Definition term_denote (vars : positive -> N) (defs : list (positive * N))
-           (x : term) : N :=
-  match x with
-  | Var n =>
-    match lookup_definition defs n with
-    | Some v => v
-    | None => vars n
-    end
-  | Value n => n
-  end.
-
-Inductive map_expr : Set :=
-  | Empty : map_expr
-  | Add   : N -> N -> N -> map_expr -> map_expr.
-
-Fixpoint map_expr_denote (vars : positive -> N) (defs : list (positive * N))
-         (m : map_expr) : M.t N :=
-  match m with
-  | Empty => M.empty N
-  | Add x y f m' => M.add (x, y) f (map_expr_denote vars defs m')
-  end.
-
-Inductive formula :=
-  | Maps    : term -> term -> term -> map_expr -> formula
-  | MapsAny : term -> term -> map_expr -> formula
-  | Impl    : formula -> formula -> formula.
-
-Fixpoint formula_denote (vars : positive -> N) (defs : list (positive * N))
-         (t : formula) : Prop :=
-  match t with
-  | Maps x y f m =>
-    M.MapsTo (term_denote vars defs x, term_denote vars defs y)
-             (term_denote vars defs f) (map_expr_denote vars defs m)
-  | MapsAny x y m =>
-    M.In (term_denote vars defs x, term_denote vars defs y)
-         (map_expr_denote vars defs m)
-  | Impl p q => formula_denote vars defs p -> formula_denote vars defs q
-  end.
-
-Inductive subterm : formula -> formula -> Prop :=
-  | Impl1 : forall t1 t2, subterm t1 (Impl t1 t2)
-  | Impl2 : forall t1 t2, subterm t2 (Impl t1 t2).
-
-Lemma subterm_wf : well_founded subterm.
-Proof.
-  constructor; intros.
-  inversion H; subst; simpl in *;
-  induction y;
-  induction t1 || induction t2;
-  simpl in *;
-  constructor; intros;
-  inversion H0; subst; clear H0;
-  try (apply IHy1; constructor);
-  try (apply IHy2; constructor).
-Defined.
-
-Section partial.
-
-Variable P : Prop.
-
-Inductive partial : Set :=
-| Proved : P -> partial
-| Uncertain : partial.
-
-Definition partialOut (x : partial) :=
+Definition partialOut {P : Prop} (x : partial P) :=
   match x return (match x with
-                  | Proved _ => P
-                  | Uncertain => True
+                  | Proved _ _  => P
+                  | Uncertain _ => True
                   end) with
-  | Proved pf => pf
-  | Uncertain => I
+  | Proved _ pf => pf
+  | Uncertain _ => I
   end.
-
-End partial.
 
 Notation "[ P ]" := (partial P) : type_scope.
 
@@ -335,229 +44,432 @@ Notation "'Reduce' v" := (if v then Yes else No) (at level 100) : partial_scope.
 Notation "x || y" := (if x then Yes else Reduce y) : partial_scope.
 Notation "x && y" := (if x then Reduce y else No) : partial_scope.
 
-Local Open Scope lazy_bool_scope.
+(**************************************************************************
+ * A term language for theorems involving FMaps
+ *)
 
-Fixpoint map_contains (vars : positive -> N) (defs : list (positive * N))
-         (x y : N) (m : map_expr) : option N :=
+Record environment := {
+  vars : positive -> N
+}.
+
+Inductive term :=
+  | Var   : positive -> term
+  | Value : N -> term.
+
+Definition term_beq (x y : term) : bool :=
+  match x, y with
+  | Var x,   Var y   => (x =? y)%positive
+  | Value x, Value y => (x =? y)%N
+  | _, _ => false
+  end.
+
+Lemma term_beq_sound x y : term_beq x y = true -> x = y.
+Proof.
+  induction x, y; simpl; intros; intuition.
+  - apply Pos.eqb_eq in H; subst; reflexivity.
+  - apply N.eqb_eq in H; subst; reflexivity.
+Defined.
+
+Lemma term_beq_neq_sound x y : term_beq x y = false -> x ≠ y.
+Proof.
+  induction x, y; simpl; intros; try discriminate.
+  - apply Pos.eqb_neq in H.
+    contradict H.
+    inversion H; subst; reflexivity.
+  - apply N.eqb_neq in H.
+    contradict H.
+    inversion H; subst; reflexivity.
+Defined.
+
+Program Definition term_eq_dec (x y : term) : {x = y} + {x ≠ y} :=
+  match x, y with
+  | Var x,   Var y   => if Pos.eq_dec x y then left _ else right _
+  | Value x, Value y => if N.eq_dec   x y then left _ else right _
+  | _, _ => right _
+  end.
+Next Obligation.
+  intuition; subst.
+  destruct y.
+    specialize (H0 p p); intuition.
+  specialize (H n n); intuition.
+Defined.
+Next Obligation.
+  split; unfold not; intros;
+  destruct H1; discriminate.
+Defined.
+Next Obligation.
+  split; unfold not; intros;
+  destruct H1; discriminate.
+Defined.
+
+Definition subst_term (x v v' : term) : term :=
+  if term_beq x v then v' else x.
+
+Fixpoint subst_all_term (x : term) (xs : list (term * term)) : term :=
+  match xs with
+  | nil => x
+  | cons (v, v') xs =>
+    subst_all_term (subst_term x v v') xs
+  end.
+
+Definition term_denote env (x : term) : N :=
+  match x with
+  | Var n => vars env n
+  | Value n => n
+  end.
+
+Inductive map_expr : Set :=
+  | Empty : map_expr
+  | Add   : term -> term -> term -> map_expr -> map_expr.
+
+Fixpoint subst_map_expr (t : map_expr) (v v' : term) : map_expr :=
+  match t with
+  | Empty => Empty
+  | Add x y f m =>
+    Add (subst_term x v v')
+        (subst_term y v v')
+        (subst_term f v v')
+        (subst_map_expr m v v')
+  end.
+
+Fixpoint subst_all_map_expr (x : map_expr) (xs : list (term * term)) : map_expr :=
+  match xs with
+  | nil => x
+  | cons (v, v') xs =>
+    subst_all_map_expr (subst_map_expr x v v') xs
+  end.
+
+Lemma subst_all_map_expr_Empty defs :
+  subst_all_map_expr Empty defs = Empty.
+Proof.
+  induction defs; simpl; auto.
+  destruct a; auto.
+Qed.
+
+Lemma subst_all_map_expr_Add defs x y f m :
+  subst_all_map_expr (Add x y f m) defs =
+  Add (subst_all_term x defs) (subst_all_term y defs)
+      (subst_all_term f defs) (subst_all_map_expr m defs).
+Proof.
+  generalize dependent m.
+  generalize dependent f.
+  generalize dependent y.
+  generalize dependent x.
+  induction defs; simpl; intros; auto.
+  destruct a.
+  rewrite IHdefs; reflexivity.
+Qed.
+
+Fixpoint map_expr_denote env (m : map_expr) : M.t N :=
   match m with
-  | Empty => None
+  | Empty => M.empty N
+  | Add x y f m' => M.add (term_denote env x, term_denote env y)
+                          (term_denote env  f) (map_expr_denote env m')
+  end.
+
+Inductive formula :=
+  | Maps : term -> term -> term -> map_expr -> formula
+  | Impl : formula -> formula -> formula.
+
+Fixpoint subst_formula (t : formula) (v v' : term) : formula :=
+  match t with
+  | Maps x y f m =>
+    Maps (subst_term x v v')
+         (subst_term y v v')
+         (subst_term f v v')
+         (subst_map_expr m v v')
+  | Impl p q => Impl (subst_formula p v v') (subst_formula q v v')
+  end.
+
+Fixpoint subst_all_formula (x : formula) (xs : list (term * term)) : formula :=
+  match xs with
+  | nil => x
+  | cons (v, v') xs =>
+    subst_all_formula (subst_formula x v v') xs
+  end.
+
+Lemma subst_all_formula_Maps defs x y f m :
+  subst_all_formula (Maps x y f m) defs =
+  Maps (subst_all_term x defs) (subst_all_term y defs)
+       (subst_all_term f defs) (subst_all_map_expr m defs).
+Proof.
+  generalize dependent m.
+  generalize dependent f.
+  generalize dependent y.
+  generalize dependent x.
+  induction defs; simpl; intros; auto.
+  destruct a.
+  rewrite IHdefs; reflexivity.
+Qed.
+
+Lemma subst_all_formula_Impl defs p q :
+  subst_all_formula (Impl p q) defs =
+  Impl (subst_all_formula p defs) (subst_all_formula q defs).
+Proof.
+  generalize dependent q.
+  generalize dependent p.
+  induction defs; simpl; intros; auto.
+  destruct a.
+  rewrite IHdefs; reflexivity.
+Qed.
+
+Fixpoint formula_denote env (t : formula) : Prop :=
+  match t with
+  | Maps x y f m =>
+    M.MapsTo (term_denote env x, term_denote env y)
+             (term_denote env f) (map_expr_denote env m)
+  | Impl p q => formula_denote env p -> formula_denote env q
+  end.
+
+Fixpoint map_expr_size (t : map_expr) : nat :=
+  match t with
+  | Empty => 1%nat
+  | Add _ _ _ m => 1%nat + map_expr_size m
+  end.
+
+Fixpoint formula_size (t : formula) : nat :=
+  match t with
+  | Maps _ _ _ m => 1%nat + map_expr_size m
+  | Impl p q => formula_size p + formula_size q
+  end.
+
+Lemma all_formulas_have_size t : (0 < formula_size t)%nat.
+Proof. induction t; simpl; omega. Qed.
+
+Lemma map_expr_size_subst_all_map_expr defs m :
+  map_expr_size (subst_all_map_expr m defs) = map_expr_size m.
+Proof.
+  induction m; simpl.
+  - rewrite subst_all_map_expr_Empty; simpl; auto.
+  - rewrite subst_all_map_expr_Add; simpl; auto.
+Qed.
+
+Lemma formula_size_subst_all_formula defs q :
+  formula_size (subst_all_formula q defs) = formula_size q.
+Proof.
+  induction q; simpl.
+  - rewrite subst_all_formula_Maps; simpl; auto.
+    rewrite map_expr_size_subst_all_map_expr; auto.
+  - rewrite subst_all_formula_Impl; simpl; auto.
+Qed.
+
+(**************************************************************************
+ * Computational decision procedure
+ *)
+
+Definition conflicted (x y : term) : bool :=
+  match x, y with
+  | Value n, Value n' => negb (N.eqb n n')
+  | _, _ => false
+  end.
+
+Definition substitution (x y : term) : option (term * term) :=
+  match x, y with
+  | Var n, Var m => if Pos.eq_dec n m then None else Some (x, y)
+  | Var _, _  => Some (x, y)
+  | _ , Var _ => Some (y, x)
+  | _, _ => None
+  end.
+
+Fixpoint substitutions (xs : list (term * term)) : list (term * term) :=
+  match xs with
+  | nil => nil
+  | cons (x, y) xs =>
+    match substitution x y with
+    | Some p => cons p (substitutions xs)
+    | None => substitutions xs
+    end
+  end.
+
+Fixpoint remove_conflicts (x y f : term) (m : map_expr) : map_expr :=
+  match m with
+  | Empty => Empty
   | Add x' y' f' m' =>
-    match N.eq_dec x x' with
-    | left _ =>
-      match N.eq_dec y y' with
-      | left _  => Some f'
-      | right _ => map_contains vars defs x y m'
-      end
-    | right _ => map_contains vars defs x y m'
-    end
+    if (conflicted x x' || conflicted y y' || conflicted f f')%bool
+    then remove_conflicts x y f m'
+    else Add x' y' f' (remove_conflicts x y f m')
   end.
 
-Lemma oops vars defs t : formula_denote vars defs t.
-Proof. Admitted.
+Lemma term_substitution_eq env t xs :
+  Forall (fun p => term_denote env (fst p) = term_denote env (snd p)) xs
+  → term_denote env (subst_all_term t (substitutions xs)) =
+    term_denote env t.
+Proof.
+  generalize dependent t.
+  induction xs; simpl; intros; auto.
+  inversion H; subst; clear H.
+  destruct a as [x y]; simpl in *.
+  destruct t; simpl; intros.
+  - destruct x, y; simpl in *; intros; auto.
+    + destruct (Pos.eq_dec p0 p1); simpl; auto.
+        rewrite IHxs; auto.
+      unfold subst_term; simpl.
+      destruct (Pos.eq_dec p p0); subst.
+        rewrite Pos.eqb_refl; simpl; auto.
+        rewrite IHxs; auto.
+      apply Pos.eqb_neq in n0; rewrite n0; simpl; auto.
+      apply IHxs; auto.
+    + unfold subst_term; simpl.
+      destruct (Pos.eq_dec p p0); subst.
+        rewrite Pos.eqb_refl; simpl; auto.
+        apply IHxs; auto.
+      apply Pos.eqb_neq in n0; rewrite n0; simpl; auto.
+      apply IHxs; auto.
+    + unfold subst_term; simpl.
+      destruct (Pos.eq_dec p p0); subst.
+        rewrite Pos.eqb_refl; simpl; auto.
+        apply IHxs; auto.
+      apply Pos.eqb_neq in n0; rewrite n0; simpl; auto.
+      apply IHxs; auto.
+    + apply IHxs; auto.
+  - destruct x, y; simpl in *; intros; try apply IHxs; auto.
+    destruct (Pos.eq_dec p p0); simpl; apply IHxs; auto.
+Qed.
 
-Definition define v v' xs :=
-  match v with
-  | Var u =>
-    match lookup_definition xs u with
-    | Some n =>
-      match N.eq_dec n v' with
-      | left _  => Some xs
-      | right _ => None
-      end
-    | None => Some (cons (u, v') xs)
-    end
-  | Value u =>
-      match N.eq_dec u v' with
-      | left _  => Some xs
-      | right _ => None
-      end
-  end.
+Lemma map_expr_substitution_eq env t xs :
+  Forall (fun p => term_denote env (fst p) = term_denote env (snd p)) xs
+    -> map_expr_denote env (subst_all_map_expr t (substitutions xs)) =
+       map_expr_denote env t.
+Proof.
+  induction t; simpl; intros.
+  - rewrite subst_all_map_expr_Empty; simpl; auto.
+  - rewrite subst_all_map_expr_Add; simpl; intros.
+    rewrite !term_substitution_eq; auto.
+    rewrite IHt; auto.
+Qed.
 
-Local Obligation Tactic := program_simpl.
+Lemma formula_substitution_eq env t xs :
+  Forall (fun p => term_denote env (fst p) = term_denote env (snd p)) xs
+    -> formula_denote env (subst_all_formula t (substitutions xs)) =
+       formula_denote env t.
+Proof.
+  induction t; simpl; intros.
+  - rewrite subst_all_formula_Maps; simpl; intros.
+    rewrite !term_substitution_eq; auto.
+    rewrite map_expr_substitution_eq; auto.
+  - rewrite subst_all_formula_Impl; simpl; intros.
+    intuition.
+    rewrite H0, H1; auto.
+Qed.
+
+Lemma terms_not_conflicted env x y :
+  term_denote env x = term_denote env y
+    -> conflicted y x = false.
+Proof.
+  destruct x, y; simpl; auto.
+  intros; subst.
+  rewrite N.eqb_refl; reflexivity.
+Qed.
 
 (* The only job of formula_forward at the moment is to accumulate variable
    definitions. *)
-Program Definition formula_forward (t : formula)
-        (vars : positive -> N) (defs : list (positive * N))
-        (hyp : formula)
-        (cont : ∀ vars' defs', [formula_denote vars' defs' t]) :
-  [formula_denote vars defs hyp -> formula_denote vars defs t] :=
+Program Definition formula_forward (t : formula) env (hyp : formula)
+        (cont : ∀ env' defs, [formula_denote env' (subst_all_formula t defs)]) :
+  [formula_denote env hyp -> formula_denote env t] :=
   match hyp with
-  | Maps x y f Empty => Yes
   | Maps x y f m =>
-    let fix go n : [formula_denote vars defs (Maps x y f n)
-                      -> formula_denote vars defs t] :=
+    let fix go n : [formula_denote env (Maps x y f n)
+                    -> formula_denote env t] :=
         match n with
-        | Empty => No
+        | Empty => Yes
         | Add x' y' f' m' =>
-          match define x x' defs with
-          | Some defs' =>
-            match define y y' defs' with
-            | Some defs'' =>
-              match define f f' defs'' with
-              | Some defs''' => cont vars defs''' || go m'
-              | None => Reduce (go m')
-              end
-            | None => Reduce (go m')
-            end
-          | None => Reduce (go m')
-          end
-        end in go m
-  | MapsAny x y Empty => Yes
-  | MapsAny x y m =>
-    let fix go n : [formula_denote vars defs (MapsAny x y n)
-                      -> formula_denote vars defs t] :=
-        match n with
-        | Empty => No
-        | Add x' y' f' m' =>
-          match define x x' defs with
-          | Some defs' =>
-            match define y y' defs' with
-            | Some defs'' => cont vars defs'' || go m'
-            | None => Reduce (go m')
-            end
-          | None => Reduce (go m')
-          end
-        end in go m
-  | Impl _ _ => Reduce (cont vars defs)
+          cont env (substitutions [(x, x'); (y, y'); (f, f')]) && go m'
+        end in Reduce (go (remove_conflicts x y f m))
+  | Impl _ _ => Reduce (cont env [])
   end.
 Next Obligation.
   simplify_maps.
-    destruct H2.
-    simpl in *.
-    subst.
-    apply oops.
-  apply oops.
-Defined.
-Next Obligation.
-  simplify_maps.
-  clear go cont.
   destruct H2.
   simpl in *.
-  subst.
-  apply oops.
+  pose proof (formula_substitution_eq env t [(x, x'); (y, y'); (f, f')]).
+  simpl in H4.
+  rewrite H4 in H; auto.
 Defined.
 Next Obligation.
+  apply H; clear H.
+  induction m; simpl in *; auto.
+  destruct (conflicted x t0) eqn:?;
+  destruct (conflicted y t1) eqn:?;
+  destruct (conflicted f t2) eqn:?;
+  simpl; simplify_maps;
+  try destruct H1;
+  simpl in *;
+  try pose proof (terms_not_conflicted _ _ _ H);
+  try pose proof (terms_not_conflicted _ _ _ H0);
+  try pose proof (terms_not_conflicted _ _ _ H2);
+  try congruence;
+  rewrite ?H, ?H0, ?H2;
   simplify_maps.
-  clear go cont.
-  destruct H2.
-  simpl in *.
-  subst.
-  apply oops.
-Defined.
-Next Obligation.
-  simplify_maps.
-  clear go cont.
-  destruct H2.
-  simpl in *.
-  subst.
-  destruct y; simpl in Heq_anonymous.
-    apply oops.
-    apply oops.
-Defined.
-Next Obligation.
-  simplify_maps.
-  clear go cont.
-  destruct H2.
-  simpl in *.
-  subst.
-  destruct y; simpl in Heq_anonymous.
-    apply oops.
-    apply oops.
-Defined.
-Next Obligation.
-  apply F.empty_in_iff in H.
-  contradiction.
-Defined.
-Next Obligation.
-  apply F.add_in_iff in H1.
-  destruct H1; auto.
-  clear go cont.
-  destruct H1.
-  simpl in *.
-  (* destruct x, y; simpl in *. *)
-  (* repeat (rewrite no_subst_formula in H; auto); auto. *)
-  apply oops.
-  apply oops.
-Defined.
-Next Obligation.
-  apply oops.
-Defined.
-Next Obligation.
-  apply F.add_in_iff in H1.
-  destruct H1; auto.
-  clear H0 go cont.
-  destruct H1.
-  simpl in *.
-  apply oops.
-Defined.
-Next Obligation.
-  apply F.add_in_iff in H1.
-  destruct H1; auto.
-  clear H0 go cont.
-  destruct H1.
-  simpl in *.
-  apply oops.
 Defined.
 
-Lemma map_contains_MapsTo vars defs x y f m :
-  Some f = map_contains vars defs x y m
-    -> M.MapsTo (x, y) f (map_expr_denote vars defs m).
+Fixpoint map_contains env (x y : term) (m : map_expr) : option term :=
+  match m with
+  | Empty => None
+  | Add x' y' f' m' =>
+    if (N.eqb (term_denote env x) (term_denote env x') &&
+        N.eqb (term_denote env y) (term_denote env y'))%bool
+    then Some f'
+    else map_contains env x y m'
+  end.
+
+Lemma map_contains_MapsTo env x y f m :
+  Some f = map_contains env x y m
+    -> M.MapsTo (term_denote env x, term_denote env y)
+                (term_denote env f) (map_expr_denote env m).
 Proof.
-  intros.
-  apply F.find_mapsto_iff.
   induction m; simpl; intros.
     discriminate.
-  simpl in *.
-  destruct (N.eq_dec x n); subst.
-    destruct (N.eq_dec y n0); subst.
-      inversion H; subst.
-      simplify_maps.
-    rewrite F.add_neq_o; auto; simpl.
-    apply not_and_implication; congruence.
-  rewrite F.add_neq_o; auto; simpl.
-  apply not_and_implication; congruence.
+  simplify_maps.
+  destruct ((term_denote env x =? term_denote env t)%N &&
+            (term_denote env y =? term_denote env t0)%N)%bool eqn:?.
+    inversion_clear H.
+    clear IHm.
+    apply andb_true_iff in Heqb.
+    destruct Heqb.
+    apply N.eqb_eq in H.
+    apply N.eqb_eq in H0.
+    intuition.
+  right.
+  apply andb_false_iff in Heqb.
+  destruct Heqb;
+  apply N.eqb_neq in H0;
+  intuition.
 Qed.
 
-Program Fixpoint formula_backward (t : formula)
-        (vars : positive -> N) (defs : list (positive * N))
-        {wf subterm t} : [formula_denote vars defs t] :=
+Program Fixpoint formula_backward (t : formula) env {measure (formula_size t)} :
+  [formula_denote env t] :=
   match t with
   | Maps x y f m =>
-    match map_contains vars defs (term_denote vars defs x)
-                       (term_denote vars defs y) m with
-    | Some f' => Reduce (N.eq_dec f' (term_denote vars defs f))
-    | None => No
-    end
-  | MapsAny x y m =>
-    match map_contains vars defs (term_denote vars defs x)
-                       (term_denote vars defs y) m with
-    | Some _ => Yes
+    match map_contains env x y m with
+    | Some f' => Reduce (term_eq_dec f' f)
     | None => No
     end
   | Impl p q =>
-    formula_forward q vars defs p
-                    (fun vars' defs' => formula_backward q vars' defs')
+    formula_forward q env p
+      (fun env' defs' => formula_backward (subst_all_formula q defs') env')
   end.
 Next Obligation.
   apply map_contains_MapsTo; auto.
 Defined.
 Next Obligation.
-  apply in_mapsto_iff.
-  eexists.
-  apply map_contains_MapsTo; auto.
-  apply Heq_anonymous.
+  rewrite formula_size_subst_all_formula; simpl.
+  apply Nat.lt_add_pos_l, all_formulas_have_size.
 Defined.
-Next Obligation.
-  destruct q; constructor.
-Defined.
-Next Obligation. apply measure_wf, subterm_wf. Defined.
 
-Definition formula_tauto : ∀ (vars : positive -> N) (t : formula),
-  [formula_denote vars nil t].
+Definition formula_tauto : ∀ env t, [formula_denote env t].
 Proof.
-  intros; refine (Reduce (formula_backward t vars nil)); auto.
+  intros; refine (Reduce (formula_backward t env)); auto.
 Defined.
+
+Lemma formula_sound env t :
+  (if formula_tauto env t then True else False) -> formula_denote env t.
+Proof.
+  unfold formula_tauto; destruct t, (formula_backward _ env); tauto.
+Qed.
+
+(**************************************************************************
+ * Environment management tactics
+ *)
 
 Ltac inList x xs :=
   match xs with
@@ -613,6 +525,10 @@ Ltac allVars xs e :=
   | _ => xs
   end.
 
+(**************************************************************************
+ * Reflection tactics
+ *)
+
 Ltac reifyValue env t :=
   match t with
   | N0 => constr:(Value N0)
@@ -626,7 +542,10 @@ Ltac reifyValue env t :=
 Ltac reifyMapTerm env t :=
   match t with
   | M.empty _ => constr:(Empty)
-  | M.add (?x, ?y) ?f ?M =>
+  | M.add (?X, ?Y) ?F ?M =>
+    let x := reifyValue env X in
+    let y := reifyValue env Y in
+    let f := reifyValue env F in
     let m := reifyMapTerm env M in
     constr:(Add x y f m)
   end.
@@ -639,11 +558,6 @@ Ltac reifyTerm env t :=
     let f := reifyValue env F in
     let m := reifyMapTerm env M in
     constr:(Maps x y f m)
-  | M.In (?X, ?Y) ?M =>
-    let x := reifyValue env X in
-    let y := reifyValue env Y in
-    let m := reifyMapTerm env M in
-    constr:(MapsAny x y m)
   | ?P -> ?Q =>
     let p := reifyTerm env P in
     let q := reifyTerm env Q in
@@ -667,44 +581,34 @@ Ltac reify :=
     let xs  := allVars tt X in
     let env := functionalize xs in
     let r1  := reifyTerm xs X in
-    change (formula_denote env nil r1)
+    change (formula_denote {| vars := env |} r1)
   end.
 
-Lemma formula_sound vars t :
-  (if formula_tauto vars t then True else False) -> formula_denote vars nil t.
-Proof.
-  unfold formula_tauto.
-  destruct t; simpl; intros.
-  - induction m; simpl in *.
-      contradiction.
-    destruct (formula_backward (Maps _ _ _ (Add _ _ _ m)) vars []) eqn:?; auto.
-    contradiction.
-  - induction m; simpl in *.
-      contradiction.
-    destruct (formula_backward (MapsAny _ _ (Add _ _ _ m)) vars []) eqn:?; auto.
-    contradiction.
-  - destruct (formula_backward (Impl _ _) vars []) eqn:?; auto.
-    contradiction.
-Qed.
+(**************************************************************************
+ * User interface tactics
+ *)
 
 Ltac solve_map := reify; apply formula_sound; vm_compute; auto.
 
-Example formula_backward_example :
-  if formula_backward
-       (Impl (Maps (Var 1%positive) (Var 2%positive) (Var 3%positive)
-                   (Add 1%N 1%N 1%N Empty))
-             (Maps (Var 1%positive) (Var 2%positive) (Var 3%positive)
-                   (Add 1%N 1%N 1%N Empty)))
-       (fun v => 9%N) nil then True else False.
-Proof.
-  vm_compute.
-  constructor.
-Qed.
+Program Instance sigT_proper {A : Type} :
+  Proper (pointwise_relation A Basics.arrow ==> Basics.arrow) (@sigT A).
+Next Obligation.
+  proper.
+  destruct X0.
+  apply X in x1.
+  exists x0.
+  assumption.
+Defined.
 
-Example map_decide_test  x y f :
-  M.MapsTo (elt:=N) (x, y) f (M.add (0%N, 0%N) 0%N (M.add (1%N, 1%N) 1%N (M.empty _))) ->
-  M.MapsTo (elt:=N) (x, y) f (M.add (0%N, 0%N) 0%N (M.add (1%N, 1%N) 1%N (M.empty _))).
-Proof. solve_map. Qed.
+Lemma find_mapsto_iff_ex {elt k m} :
+  (∃ v : elt, M.MapsTo (elt:=elt) k v m) ->
+  (∃ v : elt, M.find (elt:=elt) k m = Some v).
+Proof.
+  apply sigT_proper.
+  intros ??.
+  apply F.find_mapsto_iff.
+  assumption.
+Defined.
 
 Ltac prepare_maps :=
   repeat lazymatch goal with
@@ -720,6 +624,108 @@ Ltac prepare_maps :=
   end.
 
 Ltac map_decide := prepare_maps; solve_map.
+
+(**************************************************************************
+ * Some helper lemmas and a "traditional" FMap theorem solver
+ *)
+
+Lemma mapsto_inv : ∀ elt f g (fg : elt) x y z m,
+  M.MapsTo (f, g) fg (M.add (x, y) z m) ->
+    (x = f ∧ y = g ∧ z = fg) ∨ M.MapsTo (f, g) fg m.
+Proof.
+  intros.
+  apply add_mapsto_iffT in H.
+  destruct H; simpl in *; intuition.
+Defined.
+
+Lemma find_add_inv : ∀ f g (fg : N) x y z m,
+  M.find (f, g) (M.add (x, y) z m) = Some fg ->
+    (x = f ∧ y = g ∧ z = fg) ∨ M.find (f, g) m = Some fg.
+Proof.
+  intros.
+  destruct (N.eq_dec x f).
+    destruct (N.eq_dec y g).
+      destruct (N.eq_dec z fg).
+        subst; left; intuition.
+      contradiction n.
+      rewrite F.add_eq_o in H.
+        inversion_clear H.
+        reflexivity.
+      simpl; intuition.
+    rewrite F.add_neq_o in H; intuition.
+  rewrite F.add_neq_o in H; intuition.
+Defined.
+
+Ltac destruct_maps :=
+  repeat match goal with
+  | [ H : M.find (?X, ?Y) (M.empty _) = Some ?F |- _ ] =>
+    inversion H
+  | [ H : M.find (?X, ?Y) (M.add _ _ _) = Some ?F |- _ ] =>
+    apply find_add_inv in H;
+    (destruct H as [[? [? ?]]|]; [subst; try nomega|])
+  | [ |- ∃ v, M.find _ _ = Some v ] =>
+    vm_compute; eexists; reflexivity
+
+  | [ H : M.find _ _ = Some _ |- _ ] =>
+    apply F.find_mapsto_iff in H
+  | [ |- M.find _ _ = Some _ ] =>
+    apply F.find_mapsto_iff
+  | [ |- ∃ v, M.find _ _ = Some v ] =>
+    apply find_mapsto_iff_ex
+
+  | [ H : M.MapsTo _ _ (M.empty _) |- _ ] =>
+    contradiction (proj1 (F.empty_mapsto_iff _ _) H)
+
+  | [ H : M.MapsTo (?X, ?Y) ?F (M.add _ _ _) |- _ ] =>
+    apply mapsto_inv in H; destruct H as [[? [? ?]]|]
+
+  | [ H : ?X = ?Y |- context[M.MapsTo (?Y, _)] ] =>
+    rewrite <- H; cbn
+  | [ H : ?X = ?Y |- context[M.MapsTo (_, ?Y)] ] =>
+    rewrite <- H; cbn
+  | [ H : ?X = ?Y |- context[M.MapsTo _ ?Y] ] =>
+    rewrite <- H; cbn
+
+  | [ |- ∃ _, M.MapsTo (?X, ?Y) _ _ ] =>
+    match goal with
+      [ |- context[M.add (X, Y) ?F _ ] ] =>
+      exists F
+    end
+  | [ |- M.MapsTo (?X, ?Y) ?F (M.add (?X, ?Y) ?F _) ] =>
+    simplify_maps
+  | [ |- M.MapsTo _ _ (M.add _ _ _) ] =>
+    simplify_maps; right; split; [idtac|]
+  end;
+  try congruence.
+
+(**************************************************************************
+ * Proof of concept examples
+ *)
+
+Example formula_backward_example (x y z w : N) :
+  if formula_backward
+       (Impl (Maps (Var 1%positive) (Var 2%positive) (Var 3%positive)
+                   (Add (Value 1%N) (Value 1%N) (Var 4%positive) Empty))
+             (Maps (Var 1%positive) (Var 2%positive) (Var 3%positive)
+                   (Add (Value 1%N) (Value 1%N) (Var 4%positive) Empty)))
+       {| vars := fun p =>
+           if (p =? 1)%positive then x else
+           if (p =? 2)%positive then y else
+           if (p =? 3)%positive then z else
+           if (p =? 4)%positive then w else 9%N |}
+  then True else False.
+Proof. vm_compute; constructor. Qed.
+
+Example map_decide_test  x y f :
+  M.MapsTo (elt:=N) (x, y) f (M.add (0%N, 0%N) 0%N (M.add (1%N, 1%N) 1%N (M.empty _))) ->
+  M.MapsTo (elt:=N) (x, y) f (M.add (0%N, 0%N) 0%N (M.add (1%N, 1%N) 1%N (M.empty _))).
+Proof. solve_map. Qed.
+
+Delimit Scope fmap_scope with fmap.
+
+Notation "[map ]" := (M.empty _) (at level 9, only parsing) : fmap_scope.
+Notation "x +=> y" := (M.add x y) (at level 9, y at level 100, only parsing) : fmap_scope.
+Notation "[map  a ; .. ; b ]" := (a .. (b [map]%fmap) ..) (only parsing) : fmap_scope.
 
 Example big_problem : ∀ f g h fg gh fgh : N,
   let big :=
@@ -748,11 +754,8 @@ Example big_problem : ∀ f g h fg gh fgh : N,
 
     ;    (5, 4) +=> 7
     ;    (6, 5) +=> 8
-    (* jww (2017-07-02): With this flipped, which is wrong, map_decide works
-      (due to the 'oops' axiom, I'm guessing). *)
-    (* ;    (7, 6) +=> 9 *)
     ;    (6, 7) +=> 9
-    ;    (8, 4) +=> 9 ]%N in
+    ;    (8, 4) +=> 9 ]%N%fmap in
   M.find (elt:=N) (f,  g)  big = Some fg ->
   M.find (elt:=N) (g,  h)  big = Some gh ->
   M.find (elt:=N) (fg, h)  big = Some fgh ->
@@ -760,8 +763,10 @@ Example big_problem : ∀ f g h fg gh fgh : N,
 Proof.
   intros.
   unfold big in *; clear big.
+(*
   Time destruct_maps; try nomega. (* takes 30s *)
   Undo.
+*)
   Time map_decide.                (* takes 0.017s *)
 Qed.
 
