Lib/Datatypes.v
@@ -3,6 +3,9 @@ Set Warnings "-notation-overridden".
 Require Export Lib.Setoid.
 Require Export Lib.Tactics.
 
+Require Import Coq.NArith.NArith.
+Require Import Coq.Lists.List.
+
 Generalizable All Variables.
 Set Primitive Projections.
 Set Universe Polymorphism.
@@ -87,3 +90,88 @@ Program Definition prod_eq_dec {A B}
   | in_right => in_right
   end.
 Next Obligation. congruence. Qed.
+
+Lemma peano_rect' : ∀ P : N → Type, P 0%N → (∀ n : N, P (N.succ n)) → ∀ n : N, P n.
+Proof.
+  intros.
+  induction n using N.peano_rect.
+    apply X.
+  apply X0.
+Defined.
+
+Lemma K_dec_on_type A (x : A) (eq_dec : ∀ y : A, x = y \/ x ≠ y)
+      (P : x = x -> Type) :
+  P (eq_refl x) -> forall p:x = x, P p.
+Proof.
+  intros.
+  elim (@Eqdep_dec.eq_proofs_unicity_on A _) with x (eq_refl x) p.
+    trivial.
+  exact eq_dec.
+Qed.
+
+Lemma Pos_eq_dec' : ∀ x y : positive, x = y \/ x ≠ y.
+Proof.
+  intros.
+  destruct (Pos.eq_dec x y); auto.
+Qed.
+
+Lemma Pos_eq_dec_refl n : Pos.eq_dec n n = left (@eq_refl positive n).
+Proof.
+  destruct (Pos.eq_dec n n).
+    refine (K_dec_on_type positive n (Pos_eq_dec' n)
+              (fun x => @left _ _ x = @left _ _ (@eq_refl positive n)) _ _).
+    reflexivity.
+  contradiction.
+Qed.
+
+Lemma N_eq_dec' : ∀ x y : N, x = y \/ x ≠ y.
+Proof.
+  intros.
+  destruct (N.eq_dec x y); auto.
+Qed.
+
+Lemma N_eq_dec_refl n : N.eq_dec n n = left (@eq_refl N n).
+Proof.
+  destruct (N.eq_dec n n).
+    refine (K_dec_on_type N n (N_eq_dec' n)
+              (fun x => @left _ _ x = @left _ _ (@eq_refl N n)) _ _).
+    reflexivity.
+  contradiction.
+Qed.
+
+Lemma prod_eq_dec' :
+  ∀ (A B : Type) (A_eq_dec : ∀ x y : A, x = y ∨ x ≠ y)
+    (B_eq_dec : ∀ x y : B, x = y ∨ x ≠ y)
+    (x y : A ∧ B), x = y \/ x ≠ y.
+Proof.
+  intros.
+  destruct x, y; simpl.
+  destruct (A_eq_dec a a0); subst.
+    destruct (B_eq_dec b b0); subst.
+      left; reflexivity.
+    right; congruence.
+  right; congruence.
+Qed.
+
+Lemma prod_eq_dec_refl (A B : Type) n
+      (A_eq_dec : ∀ x y : A, x = y ∨ x ≠ y)
+      (B_eq_dec : ∀ x y : B, x = y ∨ x ≠ y) :
+  prod_eq_dec A_eq_dec B_eq_dec n n = left (@eq_refl (A ∧ B) n).
+Proof.
+  destruct (prod_eq_dec _ _ n n).
+    refine (K_dec_on_type (A ∧ B) n (prod_eq_dec' _ _ A_eq_dec B_eq_dec n)
+              (fun x => @left _ _ x = @left _ _ (@eq_refl (A ∧ B) n)) _ _).
+    reflexivity.
+  contradiction.
+Qed.
+
+Lemma length_remove A (A_eq_dec : ∀ x y : A, x = y ∨ x ≠ y) x xs :
+  (length (remove A_eq_dec x xs) <= length xs)%nat.
+Proof.
+  induction xs; auto.
+  simpl.
+  destruct (A_eq_dec x a); subst.
+    apply PeanoNat.Nat.le_le_succ_r, IHxs.
+  simpl.
+  apply le_n_S, IHxs.
+Qed.
